SortEmbeddings.v
@@ -9,6 +9,7 @@ Require Import FiniteSubstitutionSpace.
 Require Import ComputationalPathLemma.
 Require Import VarianceLabeledTree.
 Require Import Cantor.
+Require Import VectorQuantification.
 
 Module Type FiniteCountableSignatureSpec <: SignatureSpec.
   Include SignatureSpec.
@@ -320,35 +321,59 @@ Module Type TreeSpec.
 
   Declare Instance Info: LabelInfo Label.
   Declare Instance LOrder_pre: PreOrder LOrder.
-
+  
   Parameter Operation: Set.
   Parameter WellFormed: (Var -> VLTree Label EmptySet) -> Prop.
   Declare Instance Sigma: Signature (VLTree Label) Var Operation.
 
   Parameter Var_eq_dec:  forall (alpha beta: Var), { alpha = beta } + { alpha <> beta }.
-  Parameter Label_eq_dec: forall (l1 l2: Label), { l1 = l2 } + { l1 <> l2 }.  
+  Parameter Label_eq_dec: forall (l1 l2: Label), { l1 = l2 } + { l1 <> l2 }.
+  Parameter LOrder_dec: forall (l1 l2: Label), { LOrder l1 l2 } + { LOrder l1 l2 -> False }.
+
+  Declare Instance Vars_finite: Finite Var.
+  Declare Instance Labels_countable: Countable Label.
+  Parameter GroundLabel: { l : Label | labelArity l = 0 }.
 End TreeSpec.
-(* TODO:
+
 
 Module Type TreeSignatureSpec(Import Trees: TreeSpec) <: FiniteCountableSignatureSpec.
   Definition Sort: Set -> Set := VLTree Label.
   Definition Var: Set := Trees.Var.
   Definition Operation: Set := Trees.Operation.
   Definition WellFormed: (Var -> Sort EmptySet) -> Prop := Trees.WellFormed.
-  Instance SigSpec: SignatureSpecification Sort Var Operation := SigSpec.SigSpec.
-  
-  Declare Instance SigSpec: SignatureSpecification Sort Var Operation.
-End SignatureSpec.
+  Instance TreeSubst: CanSubst (VLTree Label) :=
+    {| applySubst := fun _ f t => substitute f t |}.
+  Definition TreeSubsorts: Sort EmptySet -> Sort EmptySet -> Prop :=
+    VLTreeOrder Trees.Label LOrder.
+  Instance SigSpec: SignatureSpecification Sort Var Operation :=
+    {| subsorts := VLTreeOrder Trees.Label LOrder;
+       SigmaAlgebra.Sigma := Trees.Sigma;
+       subsorts_pre := VLOrderPre _ LOrder;
+       SigmaAlgebra.Var_eq_dec := Trees.Var_eq_dec;
+       Sort_eq_dec := Tree_eq_dec _ _ Label_eq_dec (fun x => False_rect _ x);
+       subsorts_dec := VLTreeOrder_dec _ LOrder LOrder_dec;
+       SortSubst := TreeSubst |}.
+  Instance ClosedSortsCountable: Countable (Sort EmptySet) :=
+    {| toNat := VLTreeToNat _ toNat;
+       fromNat := natToVLTree _ fromNat (proj1_sig GroundLabel) (proj2_sig GroundLabel);
+       fromTo_id := natVLTree_inj toNat fromNat (proj1_sig GroundLabel) (proj2_sig GroundLabel) fromTo_id |}.       
+  Instance Vars_finite: Finite Var := Trees.Vars_finite.
+  Definition OpenSortsInhabited: Sort Var :=
+    substitute (fun devil => False_rect _ devil) (fromNat 0).
+End TreeSignatureSpec.
 
-
-Module Type TreeSortCLSignature(SigSpec: FiniteCountableSignatureSpec) <: CompatibleCLSignature.
+Module Type TreeSortCLSignature
+       (Trees: TreeSpec)
+       (SigSpec: TreeSignatureSpec(Trees)) <: CompatibleCLSignature.
   Definition Sort: Set -> Set := SigSpec.Sort.
   Definition Var: Set := SigSpec.Var.
   Definition Operation: Set := SigSpec.Operation.
   Definition WellFormed: (Var -> Sort EmptySet) -> Prop := SigSpec.WellFormed.
   Instance SigSpec: SignatureSpecification Sort Var Operation := SigSpec.SigSpec.
+
+  Inductive CtorSym : Set := BB | Dot | Label: Trees.Label -> CtorSym.
   
-  Definition ConstructorSymbol := (unit + Sort EmptySet)%type.
+  Definition ConstructorSymbol := CtorSym.
   Definition VariableSymbol := Var.
   Definition CombinatorSymbol := Operation.
   Definition VariableSymbol_eq_dec := Var_eq_dec.
@@ -356,35 +381,39 @@ Module Type TreeSortCLSignature(SigSpec: FiniteCountableSignatureSpec) <: Compat
     Definition ConstructorTaxonomy: ConstructorSymbol -> ConstructorSymbol -> Prop :=
       fun c1 c2 =>
         match c1 with
-        | inr c1 =>
+        | Label c1 =>
           match c2 with
-          | inr c2 => subsorts c1 c2
+          | Label c2 => Trees.LOrder c1 c2
           | _ => False
           end
-        | inl tt =>
+        | BB =>
           match c2 with
-          | inl tt => True
-          | inr _ => False
+          | BB => True
+          | _ => False
+          end
+        | Dot =>
+          match c2 with
+          | Dot => True
+          | _ => False
           end
         end.
     Lemma ConstructorTaxonomy_reflexive: Reflexive ConstructorTaxonomy.
     Proof.
       intro x.
-      destruct x as [ [ ] | s ].
-      - simpl; trivial.
-      - simpl.
-        generalize (subsorts_pre).
-        intro presub.
-        reflexivity.
+      destruct x as [ | | s ]; try solve [ simpl; trivial ].
+      simpl.
+      generalize (Trees.LOrder_pre).
+      intro presub.
+      reflexivity.
     Qed.
 
     Lemma ConstructorTaxonomy_transitive: Transitive ConstructorTaxonomy.
     Proof.
       intros x y z.
-      destruct x as [ [] | x ]; destruct y as [ [] | y ]; destruct z as [ [] | z ];
+      destruct x as [ | | x ]; destruct y as [ | | y ]; destruct z as [ | | z ];
         intros xy yz;
         try solve [ contradiction | trivial ].
-      generalize (subsorts_pre); intro presub.
+      generalize (Trees.LOrder_pre); intro presub.
       simpl.
       transitivity y; assumption.
     Qed.
@@ -392,11 +421,11 @@ Module Type TreeSortCLSignature(SigSpec: FiniteCountableSignatureSpec) <: Compat
     Lemma ConstructorTaxonomy_eq_dec: forall (c1 c2: ConstructorSymbol), { c1 = c2 } + { c1 <> c2 }.
     Proof.
       intros c1 c2.
-      destruct c1 as [ [] | c1 ]; destruct c2 as [ [] | c2 ];
+      destruct c1 as [ | | c1 ]; destruct c2 as [ | | c2 ];
         try solve [ left; reflexivity | right; intro devil; inversion devil ].
       generalize (SigSpec).
       intro sigspec.
-      destruct (Sort_eq_dec c1 c2);
+      destruct (Trees.Label_eq_dec c1 c2);
         [ left; apply f_equal; assumption
         | right; intro devil; inversion devil; contradiction ].
     Qed.
@@ -404,28 +433,39 @@ Module Type TreeSortCLSignature(SigSpec: FiniteCountableSignatureSpec) <: Compat
     Lemma ConstructorTaxonomy_dec: forall c1 c2, { ConstructorTaxonomy c1 c2 } + { ConstructorTaxonomy c1 c2 -> False }.
     Proof.
       intros c1 c2.
-      destruct c1 as [ [] | ]; destruct c2 as [ [] | ];
+      destruct c1 as [ | | ]; destruct c2 as [ | | ];
         try solve [ left; reflexivity | right; intro; assumption ].
-      apply subsorts_dec.
+      apply Trees.LOrder_dec.
     Qed.
 
     Definition constructorSymbolToNat (c: ConstructorSymbol): nat :=
       match c with
-      | inl tt => cantor_sum (inl 0)
-      | inr c => cantor_sum (inr (toNat c))
+      | BB => cantor_sum (inl 0)
+      | Dot => cantor_sum (inr (cantor_sum (inl 0)))
+      | Label l => cantor_sum (inr (cantor_sum (inr (toNat l))))
       end.
     Definition natToConstructorSymbol (n: nat): ConstructorSymbol :=
       match cantor_sum_inv n with
-      | inl _ => inl tt
-      | inr n => inr (fromNat n)
+      | inl _ => BB
+      | inr n =>
+        match cantor_sum_inv n with
+        | inl _ => Dot
+        | inr n => Label (fromNat n)
+        end
       end.
     Lemma fromToConstructorSymbol_id: forall c, natToConstructorSymbol (constructorSymbolToNat c) = c.
     Proof.
       intro c.
-      destruct c as [ [] | c ].
+      destruct c as [ | | l ].
       - reflexivity.
       - unfold constructorSymbolToNat.
         unfold natToConstructorSymbol.
+        rewrite (cantor_sum_inj (inr (cantor_sum (inl 0)))).
+        rewrite cantor_sum_inj.
+        reflexivity.
+      - unfold constructorSymbolToNat.
+        unfold natToConstructorSymbol.
+        rewrite cantor_sum_inj.
         rewrite cantor_sum_inj.
         rewrite fromTo_id.
         reflexivity.
@@ -433,8 +473,8 @@ Module Type TreeSortCLSignature(SigSpec: FiniteCountableSignatureSpec) <: Compat
   End ConstructorDefs.
     
   Definition Symbols: ConstructorSpecification ConstructorSymbol :=
-    {| constructorArity := fun c => match c with | inl _ => 1 | inr _ => 0 end;
-       ConstructorTaxonomy := ConstructorDefs.ConstructorTaxonomy;        
+    {| constructorArity := fun c => match c with | BB => 1 | Dot => 0 | Label l => labelArity l end;
+       ConstructorTaxonomy := ConstructorDefs.ConstructorTaxonomy;   
        CTPreorder :=
          {| PreOrder_Reflexive := ConstructorDefs.ConstructorTaxonomy_reflexive;
             PreOrder_Transitive := ConstructorDefs.ConstructorTaxonomy_transitive |};
@@ -447,56 +487,23 @@ Module Type TreeSortCLSignature(SigSpec: FiniteCountableSignatureSpec) <: Compat
   Instance Variables_finite: Finite VariableSymbol := SigSpec.Vars_finite.
   Definition ClosedSortsInhabited: Sort EmptySet := fromNat 0.
   Definition OpenSortsInhabited: Sort Var := SigSpec.OpenSortsInhabited.
-  Definition BlackBox : ConstructorSymbol := inl tt.
+  Definition BlackBox : ConstructorSymbol := BB.
   Lemma BlackBoxArity: @constructorArity _ Symbols BlackBox = 1.
   Proof.
     reflexivity.
   Qed.
-End SortConstructorCLSignature.
+End TreeSortCLSignature.
 
-Module Type CountableClosedSortSignatureSpec.
-  Include SignatureSpec with Definition Var := EmptySet.
-  Declare Instance ClosedSortsCountable: Countable (Sort EmptySet).
-  Parameter applySubst_eq: forall S s, applySubst S s = s.
-End CountableClosedSortSignatureSpec.
+Module Type MakeTreeSortCLSignature(Trees: TreeSpec).
+  Declare Module SigSpec: TreeSignatureSpec(Trees).
+  Declare Module Signature: TreeSortCLSignature(Trees)(SigSpec).
+End MakeTreeSortCLSignature.
 
-Module Type FiniteCountableFromCountableClosedSortSignatureSpec
-       (SigSpec: CountableClosedSortSignatureSpec) <: FiniteCountableSignatureSpec.
-  Definition Sort: Set -> Set := SigSpec.Sort.
-  Definition Var: Set := SigSpec.Var.
-  Definition Operation: Set := SigSpec.Operation.
-  Definition WellFormed: (Var -> Sort EmptySet) -> Prop := SigSpec.WellFormed.
-  Instance SigSpec: SignatureSpecification Sort Var Operation := SigSpec.SigSpec.
-  Instance ClosedSortsCountable: Countable (Sort EmptySet) := SigSpec.ClosedSortsCountable.
-  Instance Vars_finite: Finite Var :=
-    {| cardinality := 0;
-       toFin := fun devil => False_rect _ devil;
-       fromFin := fun devil =>
-                    match devil in Fin.t n return 0 = n -> EmptySet with
-                    | Fin.F1 =>
-                      fun devil' =>
-                        match devil' in _ = n return match n with | 0 => True | _ => False end with
-                        | eq_refl => I
-                        end  
-                    | Fin.FS _ =>
-                      fun devil' =>
-                        match devil' in _ = n return match n with | 0 => True | _ => False end with
-                        | eq_refl => I
-                        end
-                    end eq_refl;
-       fromToFin_id := fun devil => False_rect _ devil |}.
-  Definition OpenSortsInhabited: Sort Var := fromNat 0.
-End FiniteCountableFromCountableClosedSortSignatureSpec.
+(* In progress
 
-Module Type MakeClosedSortCLSignature(SigSpec: CountableClosedSortSignatureSpec).
-  Declare Module SigSpec' : FiniteCountableFromCountableClosedSortSignatureSpec(SigSpec).
-  Declare Module Signature : SortConstructorCLSignature(SigSpec').
-End MakeClosedSortCLSignature.
-
-
-Module Type ProperConstantEmbedding
-       (Import SigSpec: CountableClosedSortSignatureSpec)
-       (Import MakeSignature: MakeClosedSortCLSignature(SigSpec))
+Module Type ProperTreeSortEmbedding
+       (Import Trees: TreeSpec)
+       (Import MakeSignature: MakeTreeSortCLSignature(Trees))
        (Import Types: IntersectionTypes(MakeSignature.Signature))
 <: WithProperEmbedding(MakeSignature.Signature)(Types).
   
@@ -508,27 +515,200 @@ Module Type ProperConstantEmbedding
 
   Module Proper.
     Import Signature.
-    Definition embedS (s: Sort EmptySet) := ConstScheme (inr s) (nil _).
-    Definition unembedS (ts: TypeScheme (VariableSymbol := EmptySet)): Sort EmptySet :=
+
+    Definition ClosedArrowScheme (src tgt: @TypeScheme EmptySet): @TypeScheme EmptySet :=
+      Skeleton (PT_Arrow src tgt).
+
+    Definition ClosedConstScheme
+               (c: ConstructorSymbol)
+               (xs: t (@TypeScheme EmptySet) (constructorArity c)): @TypeScheme EmptySet :=
+      Skeleton (PT_Const c xs).      
+    
+    Fixpoint closedEmbedS_variance (s: Sort EmptySet) (v: Variance) {struct s}: @TypeScheme EmptySet :=
+      match s with
+      | Node _ _ l xs =>
+        match v with
+        | Co =>
+          ClosedArrowScheme (ClosedArrowScheme
+                               (ClosedConstScheme (Label l)
+                                                  (map2 (fun x v => closedEmbedS_variance x (successorVariance l v))
+                                                        xs
+                                                        (positions (labelArity l))))
+                               (ClosedConstScheme Dot (nil _)))
+                            (ClosedConstScheme Dot (nil _))
+        | Contra =>
+          ClosedArrowScheme (ClosedArrowScheme
+                               (ClosedConstScheme Dot (nil _))
+                               (ClosedConstScheme (Label l)
+                                                  (map2 (fun x v => closedEmbedS_variance x (successorVariance l v))
+                                                        xs
+                                                        (positions (labelArity l)))))
+                            (ClosedConstScheme Dot (nil _))
+        | In =>
+          ClosedArrowScheme (ClosedArrowScheme
+                               (ClosedConstScheme (Label l)
+                                                  (map2 (fun x v => closedEmbedS_variance x (successorVariance l v))
+                                                        xs
+                                                        (positions (labelArity l))))
+                               (ClosedConstScheme (Label l)
+                                                  (map2 (fun x v => closedEmbedS_variance x (successorVariance l v))
+                                                        xs
+                                                        (positions (labelArity l)))))
+                            (ClosedConstScheme Dot (nil _))
+        end
+      | Hole _ _ alpha => False_rect _ alpha
+      end.
+    
+    Fixpoint openEmbedS_variance (s: Sort Var) (v: Variance) {struct s}: TypeScheme :=
+      match s with
+      | Node _ _ l xs =>
+        match v with
+        | Co =>
+          ArrowScheme (ArrowScheme
+                         (ConstScheme (Label l)
+                                      (map2 (fun x v => openEmbedS_variance x (successorVariance l v))
+                                            xs
+                                            (positions (labelArity l))))
+                         (ConstScheme Dot (nil _)))
+                      (ConstScheme Dot (nil _))
+        | Contra =>
+          ArrowScheme (ArrowScheme
+                         (ConstScheme Dot (nil _))
+                         (ConstScheme (Label l)
+                                      (map2 (fun x v => openEmbedS_variance x (successorVariance l v))
+                                            xs
+                                            (positions (labelArity l)))))
+                      (ConstScheme Dot (nil _))
+        | In =>
+          ArrowScheme (ArrowScheme
+                         (ConstScheme (Label l)
+                                      (map2 (fun x v => openEmbedS_variance x (successorVariance l v))
+                                            xs
+                                            (positions (labelArity l))))
+                         (ConstScheme (Label l)
+                                      (map2 (fun x v => openEmbedS_variance x (successorVariance l v))
+                                            xs
+                                            (positions (labelArity l)))))
+                      (ConstScheme Dot (nil _))
+        end
+      | Hole _ _ alpha => Types.Var alpha
+      end.
+    
+    Definition closedEmbedS (s: Sort EmptySet) := closedEmbedS_variance s Co.
+    Definition openEmbedS (s: Sort Var) := openEmbedS_variance s Co.
+    
+    Fixpoint closedUnembedS (ts: TypeScheme (VariableSymbol := EmptySet)): Sort EmptySet :=
       match ts with
-      | Skeleton (PT_Const (inr C) _) => C
+      | Skeleton (PT_Arrow (Skeleton (PT_Arrow (Skeleton (PT_Const (Label l) xs)) _)) _) =>
+        Node _ _ l (map closedUnembedS xs)
+      | Skeleton (PT_Arrow (Skeleton (PT_Arrow _ (Skeleton (PT_Const (Label l) xs)))) _) =>
+        Node _ _ l (map closedUnembedS xs)
+      | _ => ClosedSortsInhabited
+      end.
+    
+    Fixpoint openUnembedS (ts: TypeScheme (VariableSymbol := Var)): Sort Var :=
+      match ts with
+      | Skeleton (PT_Arrow (Skeleton (PT_Arrow (Skeleton (PT_Const (Label l) xs)) _)) _) =>
+        Node _ _ l (map openUnembedS xs)
+      | Skeleton (PT_Arrow (Skeleton (PT_Arrow _ (Skeleton (PT_Const (Label l) xs)))) _) =>
+        Node _ _ l (map openUnembedS xs)
+      | Types.Var alpha => Hole _ _ alpha
       | _ => OpenSortsInhabited
       end.
 
     Instance ClosedEmbedding : Embedding EmptySet :=
-      {| embed := embedS; unembed := unembedS |}.
+      {| embed := closedEmbedS; unembed := closedUnembedS |}.
+    Instance OpenEmbedding : Embedding Var :=
+      {| embed := openEmbedS; unembed := openUnembedS |}.
 
-    Lemma injectivity: forall (s: Sort EmptySet), unembed (embed s) = s.
+    Lemma openInjectivity: forall (s: Sort Var), unembed (embed s) = s.
     Proof.
-      intro; reflexivity.
+      intro s.
+      unfold embed.
+      unfold unembed.
+      simpl.
+      unfold openEmbedS.
+      generalize (Co).
+      induction s as [ alpha | l successors IH ] using VLTree_rect'.
+      - intro v; simpl; destruct v; reflexivity.
+      - intro v.
+        assert (successors_eq:
+                  map openUnembedS
+                      (map2 (fun x v => openEmbedS_variance x (successorVariance l v))
+                            successors (positions (labelArity l))) = successors).
+        { revert successors IH.
+          generalize (successorVariance l).
+          generalize (labelArity l).
+          intros arity succVar successors IH'.
+          generalize (Forall_nth _ _ (ForAll'Forall _ _ IH')).
+          intro IH; clear IH'.
+          rewrite (map_map2_fg).
+          induction successors as [ | successor n successors IH' ].
+          - reflexivity.
+          - simpl.
+            rewrite (IH Fin.F1 _).
+            simpl.
+            apply f_equal.
+            rewrite <- (IH' (fun k => succVar (Fin.FS k)) (fun k => IH (Fin.FS k))) at 2.
+            rewrite <- (map_id successors (fun x => x) (fun x => eq_refl)).
+            rewrite <- (map_id (positions n) (fun x => x) (fun x => eq_refl)) at 2.
+            rewrite map2_map_fg.
+            rewrite map2_map_fg.
+            reflexivity. }
+        destruct v; simpl; rewrite successors_eq; reflexivity.
     Qed.
 
-    Instance ClosedInjectiveEmbedding: InjectiveEmbedding EmptySet :=
-      {| Embed := ClosedEmbedding; unembedEmbed := injectivity |}.
-
-    Lemma embed_respectful: forall s s', subsorts s s' -> freeze (embed s) <= freeze (embed s').
+    Lemma closedInjectivity: forall (s: Sort EmptySet), unembed (embed s) = s.
     Proof.
-      intros s s' s_le.
+      intro s.
+      unfold embed.
+      unfold unembed.
+      simpl.
+      unfold closedEmbedS.
+      generalize (Co).
+      induction s as [ | l successors IH ] using VLTree_rect'.
+      - contradiction.
+      - intro v.
+        assert (successors_eq:
+                  map closedUnembedS
+                      (map2 (fun x v => closedEmbedS_variance x (successorVariance l v))
+                            successors (positions (labelArity l))) = successors).
+        { revert successors IH.
+          generalize (successorVariance l).
+          generalize (labelArity l).
+          intros arity succVar successors IH'.
+          generalize (Forall_nth _ _ (ForAll'Forall _ _ IH')).
+          intro IH; clear IH'.
+          rewrite (map_map2_fg).
+          induction successors as [ | successor n successors IH' ].
+          - reflexivity.
+          - simpl.
+            rewrite (IH Fin.F1 _).
+            simpl.
+            apply f_equal.
+            rewrite <- (IH' (fun k => succVar (Fin.FS k)) (fun k => IH (Fin.FS k))) at 2.
+            rewrite <- (map_id successors (fun x => x) (fun x => eq_refl)).
+            rewrite <- (map_id (positions n) (fun x => x) (fun x => eq_refl)) at 2.
+            rewrite map2_map_fg.
+            rewrite map2_map_fg.
+            reflexivity. }
+        destruct v; simpl; rewrite successors_eq; reflexivity.
+    Qed.
+    
+    Instance ClosedInjectiveEmbedding: InjectiveEmbedding EmptySet :=
+      {| Embed := ClosedEmbedding; unembedEmbed := closedInjectivity |}.
+    Instance OpenInjectiveEmbedding: InjectiveEmbedding Var :=
+      {| Embed := OpenEmbedding; unembedEmbed := openInjectivity |}.
+    (*Lemma embed_respectful: forall s s', subsorts s s' -> freeze (embed s) <= freeze (embed s').
+    Proof.
+      intro s.
+      induction s as [ | l successors IH ] using VLTree_rect'; [ contradiction | ].
+      intros s' s_le.
+      destruct s'; [ | contradiction ].
+      simpl.
+      apply ST_CoContra; [ | reflexivity ].
+      
+      inversion s_le.
       apply (ST_Ax (inr s) (inr s') eq_refl); [ assumption | apply Forall2_nil ].
     Qed.
 
@@ -551,21 +731,174 @@ Module Type ProperConstantEmbedding
       rewrite injectivity.
       rewrite injectivity.
       assumption.
-    Qed.
+    Qed.*)
 
     Lemma embed_Path: forall s, Path (freeze (embed s)).
     Proof.
       intros.
+      destruct s; [ | contradiction ].
+      simpl.
+      apply Path_Arr.
       apply Path_Const.
       apply PathArgs_nil.
     Qed.
 
-    Lemma embedApply: forall S s, freeze (embed (applySubst S s)) = Apply (embedSubst S) (embed s).
+    (*Lemma applyEq:
+      forall S s v,
+        freeze (closedEmbedS (substitute S s)) = Apply (embedSubst S) (openEmbedS s) ->
+        freeze (closedEmbedS_variance (substitute S s) v) =
+        Apply (embedSubst S) (openEmbedS_variance s v).
     Proof.
       intros S s.
-      simpl.
-      rewrite applySubst_eq.
-      reflexivity.
+      induction s as [ alpha | l successors IH ] using VLTree_rect'.
+      - unfold embedSubst.
+        intro v.
+        simpl.
+        destruct v.
+        + simpl.
+          unfold closedEmbedS.
+          intro; reflexivity.
+        + simpl.
+          unfold closedEmbedS.*)
+
+    Lemma embedApply_Var: forall S alpha, freeze (embed (applySubst S (Hole _ _ alpha))) =
+                                     Apply (embedSubst S) (embed (Hole _ _ alpha)).
+    Proof.
+      intros S alpha; reflexivity.
+    Qed.
+
+    Require Import Coq.Arith.Wf_nat.
+
+    Lemma embedApply: forall S s, freeze (embed (applySubst S s)) =
+                                     Apply (embedSubst S) (embed s).
+    Proof.
+      intros S s.
+      unfold embed.
+      unfold embedSubst.
+      unfold ClosedEmbedding.
+      unfold OpenEmbedding.
+      unfold embed.
+      unfold closedEmbedS.
+      unfold openEmbedS.
+      generalize Co.      
+      apply (fun IH => Fix (well_founded_ltof _ (VLTree_size _ _))
+                        (fun s => forall v, freeze (closedEmbedS_variance (applySubst S s) v) =
+                                    Apply _ (openEmbedS_variance s v)) IH s).
+      clear s; intro s.
+      destruct s as [ l successors | ].
+      - intros IH v.
+        destruct v.
+        + simpl.
+          apply f_equal2; [ | reflexivity ].
+          apply f_equal2; [ | reflexivity ].
+          apply f_equal.
+          rewrite map_map2_fg.
+          rewrite map_map2_fg.
+          rewrite <- (map_id (positions (labelArity l)) (fun x => x) (fun x => eq_refl)) at 1.
+          rewrite map2_map_fg.
+          revert successors IH.
+          generalize (successorVariance l).
+          unfold ltof.
+          unfold constructorArity.
+          simpl.
+          generalize (labelArity l).
+          intros arity succVar successors successorPrfs.
+          generalize Co.
+          induction successorPrfs as [ | n successor successors prf prfs IH ].
+          * reflexivity.
+          * intro v.
+            simpl.
+            rewrite <- (map_id successors (fun x => x) (fun x => eq_refl)).
+            rewrite map2_map_fg.
+            rewrite map2_map_fg.
+            rewrite (IH (fun k => succVar (Fin.FS k)) v).
+            apply (f_equal (fun x => cons _ x _ _)).
+            destruct successor.
+            
+      
+      assert (notHole: forall alpha, Node _ _ l xs <> Hole _ _ alpha).
+      { intros alpha devil; inversion devil. }     
+      unfold embed.
+      unfold embedSubst.
+      unfold ClosedEmbedding.
+      unfold OpenEmbedding.
+      unfold embed.
+      unfold closedEmbedS.
+      unfold openEmbedS.
+      generalize Co.      
+      induction (Node _ _ l xs) as [ alpha | l' successors IH ] using VLTree_rect'.
+      - destruct (notHole alpha eq_refl).
+      - clear l xs notHole.
+        simpl.
+        intro v.
+        destruct v.
+        + simpl.
+          apply f_equal2; [ | reflexivity ].
+          apply f_equal2; [ | reflexivity ].
+          apply f_equal.
+          rewrite map_map2_fg.
+          rewrite map_map2_fg.
+          rewrite <- (map_id (positions (labelArity l')) (fun x => x) (fun x => eq_refl)) at 1.
+          rewrite map2_map_fg.
+          generalize (ForAll'Forall _ _ IH).
+          clear IH.
+          revert successors.
+          generalize (successorVariance l').
+          unfold constructorArity.
+          simpl.
+          generalize (labelArity l').
+          intros arity succVar successors successorPrfs.
+          generalize Co.
+          induction successorPrfs as [ | n successor successors prf prfs IH ].
+          * reflexivity.
+          * intro v.
+            simpl.
+            rewrite <- (map_id successors (fun x => x) (fun x => eq_refl)).
+            rewrite map2_map_fg.
+            rewrite map2_map_fg.
+            rewrite (IH (fun k => succVar (Fin.FS k)) v).
+            apply (f_equal (fun x => cons _ x _ _)).
+            destruct successor.
+            { rewrite prf.
+              - reflexivity.
+                reflexivity.
+              reflexivity.
+            reflexivity.
+        
+
+        intro v.
+        destruct v.
+        + simpl.
+          apply f_equal2; [ | reflexivity ].
+          apply f_equal2; [ | reflexivity ].
+          apply f_equal.
+          rewrite map_map2_fg.
+          rewrite map_map2_fg.
+          rewrite <- (map_id (positions (labelArity l)) (fun x => x) (fun x => eq_refl)) at 1.
+          rewrite map2_map_fg.
+          generalize (ForAll'Forall _ _ IH).
+          clear IH.
+          revert successors.
+          generalize (successorVariance l).
+          unfold constructorArity.
+          simpl.
+          generalize (labelArity l).
+          intros arity succVar successors successorPrfs.
+          induction successorPrfs as [ | n successor successors prf prfs IH ].
+          * reflexivity.
+          * simpl.
+            rewrite <- (map_id successors (fun x => x) (fun x => eq_refl)).
+            rewrite map2_map_fg.
+            rewrite map2_map_fg.
+            rewrite (IH (fun k => succVar (Fin.FS k))).
+            apply (f_equal (fun x => cons _ x _ _)).
+            rewrite prf.
+            reflexivity.
+      + 
+        
+      
+      
+            
     Qed.
 
     Lemma unembedApply: forall S tau,
@@ -593,44 +926,4 @@ Module Type ProperConstantEmbedding
        unembedApply := Proper.unembedApply |}.       
 End ProperConstantEmbedding.
 
-Module Type ConstantFiniteWellFormedPredicate
-       (Import SigSpec: CountableClosedSortSignatureSpec)
-       (Import MakeSignature: MakeClosedSortCLSignature(SigSpec))
-       (Import Types: IntersectionTypes(MakeSignature.Signature))
-<: FiniteWellFormedPredicate(MakeSignature.Signature)(Types)
-<: DecidableWellFormedPredicate(MakeSignature.Signature)(Types).
-  Definition WellFormed: Substitution -> Prop := fun S => forall alpha, S alpha = omega.
-  Definition SubstitutionSpace : Set := unit.
-  Definition SubstitutionSpace_sound: SubstitutionSpace -> { S : Substitution | WellFormed S } :=
-    fun _ => exist _ (fun _ => omega) (fun alpha => eq_refl).
-  Definition SubstitutionSpace_complete: { S : Substitution | WellFormed S } -> SubstitutionSpace :=
-    fun _ => tt.
-  Lemma SubstitutionSpace_eq:
-    forall WFS alpha, proj1_sig (SubstitutionSpace_sound (SubstitutionSpace_complete WFS)) alpha =
-                 proj1_sig WFS alpha.
-  Proof.
-    intros WFS alpha; simpl.
-    rewrite (proj2_sig WFS alpha).
-    reflexivity.
-  Qed.
-  Instance SubstitutionSpace_finite: Finite SubstitutionSpace :=
-    {| cardinality := 1;
-       toFin := fun _ => Fin.F1;
-       fromFin := fun _ => tt;
-       fromToFin_id := fun x => match x with | tt => eq_refl end |}.
-  Lemma WF_dec: forall S, { WellFormed S } + { ~ WellFormed S }.
-  Proof.
-    intro S; left; intro alpha.
-    contradiction.
-  Qed.
-
-  Lemma WF_ext: forall S S', (forall alpha, S alpha = S' alpha) -> WellFormed S -> WellFormed S'.
-  Proof.
-    intros S S' S_eq WF_S.
-    intro alpha.
-    rewrite <- (S_eq alpha).
-    apply WF_S.
-  Qed.
-   
-End ConstantFiniteWellFormedPredicate.                  
 *)
